<?xml version="1.0" encoding="utf-8" ?>
<rdf:RDF xmlns:rdf="http://www.w3.org/1999/02/22-rdf-syntax-ns#"
         xmlns:adms="http://www.w3.org/ns/adms#"
         xmlns:skos="http://www.w3.org/2004/02/skos/core#"
         xmlns:rdfs="http://www.w3.org/2000/01/rdf-schema#"
         xmlns:dc="http://purl.org/dc/terms/">

  <skos:ConceptScheme rdf:about="http://data.europa.eu/eif/">
    <rdfs:label>The European Interoperability Framework (EIF)</rdfs:label>
    <dc:creator>Natasa Sofou</dc:creator>
    <dc:description>Linked data representation of the EIF</dc:description>
    <skos:prefLabel xml:lang="en">The European Interoperability Framework (EIF)</skos:prefLabel>
    <skos:definition xml:lang="en">A set of principles intended to establish general behaviors on interoperability;
    </skos:definition>
    <skos:scopeNote xml:lang="en">The EIF is meant to be a generic framework applicable to all public administrations in
      the EU. It lays out the basic conditions for achieving interoperability, acting as the common denominator for
      relevant initiatives at all levels including European, national, regional and local, embracing public
      administrations, citizens and businesses. This document is addressed to all those involved in defining, designing,
      developing and delivering European public services.
    </skos:scopeNote>
    <skos:hasTopConcept rdf:resource="http://data.europa.eu/Principle"/>
    <skos:hasTopConcept rdf:resource="http://data.europa.eu/Recommendation"/>
    <skos:hasTopConcept rdf:resource="http://data.europa.eu/Layer"/>
    <skos:hasTopCOncept rdf:resource="http://data.europa.eu/Model"/>
  </skos:ConceptScheme>

  <skos:Concept rdf:about="http://data.europa.eu/UP1">
    <skos:prefLabel xml:lang="en">Underlying Principle 1: subsidiarity and proportionality</skos:prefLabel>
    <skos:altLabel xml:lang="en">UP1</skos:altLabel>
    <skos:definition xml:lang="en">The subsidiarity principle requires EU decisions to be taken as closely as possible
      to the citizen. The EU does not take action unless this is more effective than the same action taken at national
      level. The proportionality principle limits EU actions to what is necessary to achieve the objectives of the
      Treaties.
    </skos:definition>
    <skos:broader rdf:resource="http://data.europa.eu/Principle"/>
    <skos:inScheme rdf:resource="http://data.europa.eu/eif/"/>
    <adms:identifier>4</adms:identifier>
  </skos:Concept>

  <skos:Concept rdf:about="http://data.europa.eu/UP2">
    <skos:prefLabel xml:lang="en">Underlying Principle 2: openess</skos:prefLabel>
    <skos:altLabel xml:lang="en">UP2</skos:altLabel>
    <skos:definition xml:lang="en">The concept of openness mainly relates to data, specifications and software. Open
      government data (here simply referred ‘open data’) refers to the idea that all public data should be freely
      available for use and reuse by others, unless restrictions apply e.g. for protection of personal data,
      confidentiality, or intellectual property rights. Public administrations collect and generate huge amounts of
      data. The Directive on the reuse of public sector information (PSI)7 encourages Member States to make public
      information available for access and reuse as open data. The INSPIRE Directive8 requires, in addition, sharing of
      spatial datasets and services between public authorities with no restrictions or practical obstacles to its reuse.
      This data should be published with as few restrictions as possible and clear licences for its use to allow better
      scrutiny of administrations’ decision-making processes and realise transparency in practice.
    </skos:definition>
    <skos:broader rdf:resource="http://data.europa.eu/Principle"/>
    <skos:inScheme rdf:resource="http://data.europa.eu/eif/"/>
    <adms:identifier>5</adms:identifier>
  </skos:Concept>

  <skos:Concept rdf:about="http://data.europa.eu/UP3">
    <skos:prefLabel xml:lang="en">Underlying Principle 3: transparency</skos:prefLabel>
    <skos:altLabel xml:lang="en">UP3</skos:altLabel>
    <skos:definition xml:lang="en">(1). Enabling visibility inside the administrative environment of a public
      administration. This is about allowing other public administrations, citizens and businesses to view and
      understand administrative rules, processes11, data, services and decision-making (2). Ensuring availability of
      interfaces with internal information systems. Public administrations operate a large number of what are often
      heterogeneous and disparate information systems in support of their internal processes. Interoperability depends
      on ensuring the availability of interfaces to these systems and the data they handle. In turn, interoperability
      facilitates reuse of systems and data, and enables these to be integrated into larger systems. (3). Securing the
      right to the protection of personal data, by respecting the applicable legal framework for the large volumes of
      personal data of citizens, held and managed by Public administrations.
    </skos:definition>
    <skos:broader rdf:resource="http://data.europa.eu/Principle"/>
    <skos:inScheme rdf:resource="http://data.europa.eu/eif/"/>
    <adms:identifier>6</adms:identifier>
  </skos:Concept>

  <skos:Concept rdf:about="http://data.europa.eu/UP4">
    <skos:prefLabel xml:lang="en">Underlying Principle 4: reusability</skos:prefLabel>
    <skos:altLabel xml:lang="en">UP4</skos:altLabel>
    <skos:definition xml:lang="en">Interfaces, standards), information and data, is an enabler of interoperability and
      improves quality because it extends operational use, as well as saving money and time. This makes it a major
      contributor to the development of a digital single market in the EU. Some EU standards and specifications also
      exist in the DIFs and should be applied more widely. For example, the INSPIRE Directive sets out interoperability
      standards for addresses, cadastres, roads and many other data topics of relevance to many public administrations.
      These existing standards and specifications can and should be used more widely beyond the domain for which they
      were originally developed.
    </skos:definition>
    <skos:broader rdf:resource="http://data.europa.eu/Principle"/>
    <skos:inScheme rdf:resource="http://data.europa.eu/eif/"/>
    <adms:identifier>7</adms:identifier>
  </skos:Concept>

  <skos:Concept rdf:about="http://data.europa.eu/UP5">
    <skos:prefLabel xml:lang="en">Underlying Principle 5: technological neutrality and data portability</skos:prefLabel>
    <skos:altLabel xml:lang="en">UP5</skos:altLabel>
    <skos:definition>When establishing European public services, public administrations should focus on functional needs
      and defer decisions on technology as long as possible in order to minimise technological dependencies, to avoid
      imposing specific technical implementations or products on their constituents. Public administrations should
      provide for access and reuse of their public services and data irrespective of specific technologies or
      products.The functioning of the digital single market requires data to be easily transferable among different
      systems to avoid lock-in, support the free movement of data. This requirement relates to data portability - the
      ability to move and reuse data easily among different applications and systems, which becomes even more
      challenging in cross-border scenarios.
    </skos:definition>
    <skos:broader rdf:resource="http://data.europa.eu/Principle"/>
    <skos:inScheme rdf:resource="http://data.europa.eu/eif/"/>
    <adms:identifier>8</adms:identifier>
  </skos:Concept>

  <skos:Concept rdf:about="http://data.europa.eu/UP6">
    <skos:prefLabel xml:lang="en">Underlying Principle 6: user centricity</skos:prefLabel>
    <skos:altLabel xml:lang="en">UP6</skos:altLabel>
    <skos:definition xml:lang="en">Users’ needs should be considered when determining which public services should be
      provided and how they should be delivered., n accordance with the following expectations: (1). A multi-channel
      service delivery approach, meaning the availability of alternative channels, physical and digital, to access a
      service, is an important part of public service design, as users may prefer different channels depending on the
      circumstances and their needs; (2). A single point of contact should be made available to users, to hide internal
      administrative complexity and facilitate access to public services, e.g. when multiple bodies have to work
      together to provide a public service; (3). Users’ feedback should be systematically collected, assessed and used
      to design new public services and to further improve existing ones; (4). As far as possible, under the legislation
      in force, users should be able to provide data once only, and administrations should be able to retrieve and share
      this data to serve the user, in accordance with data protection rule (5). Users should be asked to provide only
      the information that is absolutely necessary to obtain a given public service.
    </skos:definition>
    <skos:broader rdf:resource="http://data.europa.eu/Principle"/>
    <skos:inScheme rdf:resource="http://data.europa.eu/eif/"/>
    <adms:identifier>9</adms:identifier>
  </skos:Concept>

  <skos:Concept rdf:about="http://data.europa.eu/UP7">
    <skos:prefLabel xml:lang="en">Underlying Principle 7: inclusion and accessibility</skos:prefLabel>
    <skos:altLabel xml:lang="en">UP7</skos:altLabel>
    <skos:definition xml:lang="en">Inclusion is about enabling everyone to take full advantage of the opportunities
      offered by new technologies to access and make use of European public services, overcoming social and economic
      divides and exclusion. Accessibility ensures that people with disabilities, the elderly and other disadvantaged
      groups can use public services at service levels comparable to those provided to other citizens.
    </skos:definition>
    <skos:broader rdf:resource="http://data.europa.eu/Principle"/>
    <skos:inScheme rdf:resource="http://data.europa.eu/eif/"/>
    <adms:identifier>10</adms:identifier>
  </skos:Concept>

  <skos:Concept rdf:about="http://data.europa.eu/UP8">
    <skos:prefLabel xml:lang="en">Underlying Principle 8: security and privacy</skos:prefLabel>
    <skos:altLabel xml:lang="en">UP8</skos:altLabel>
    <skos:definition xml:lang="en">Citizens and businesses must be confident that when they interact with public
      authorities they are doing so in a secure and trustworthy environment and in full compliance with relevant
      regulations, e.g. the Regulation and Directive on data protection16, and the Regulation on electronic
      identification and trust services17. Public administrations must guarantee the citizens’ privacy, and the
      confidentiality, authenticity, integrity and non-repudiation of information provided by citizens and businesses.
    </skos:definition>
    <skos:broader rdf:resource="http://data.europa.eu/Principle"/>
    <skos:inScheme rdf:resource="http://data.europa.eu/eif/"/>
    <adms:identifier>11</adms:identifier>
  </skos:Concept>

  <skos:Concept rdf:about="http://data.europa.eu/UP9">
    <skos:prefLabel xml:lang="en">Underlying Principle 9: multilingualism</skos:prefLabel>
    <skos:altLabel xml:lang="en">UP9</skos:altLabel>
    <skos:definition xml:lang="en">European public services can potentially be used by anyone in any Member State. So
      multilingualism needs to be carefully considered when designing them. Citizens across Europe often have problems
      in accessing and using digital public services if these are not available in the languages they speak. A balance
      needs to be found between the expectations of citizens and businesses to be served in their own language(s) or
      their preferred language(s) and the ability of Member States’ public administrations to offer services in all
      official EU languages. A suitable balance could be that European public services are available in the languages of
      the expected end-users, i.e. the number of languages is decided on the basis of users’ needs, such as the level to
      which the service is critical for the implementation of the digital single market or national policies, or the
      size of the relevant audience. Multilingualism comes into play not just in the user interface, but at all levels
      in the design of European public services. For example, the choices made on data representation in an electronic
      database should not limit its ability to support different languages.he multilingual aspect of interoperability
      becomes also relevant when a public service requires exchanges between information systems across language
      boundaries, as the meaning of the information exchanged must be preserved.
    </skos:definition>
    <skos:broader rdf:resource="http://data.europa.eu/Principle"/>
    <skos:inScheme rdf:resource="http://data.europa.eu/eif/"/>
    <adms:identifier>12</adms:identifier>
  </skos:Concept>

  <skos:Concept rdf:about="http://data.europa.eu/UP10">
    <skos:prefLabel xml:lang="en">Underlying Principle 10: administrative simplification</skos:prefLabel>
    <skos:altLabel xml:lang="en">UP10</skos:altLabel>
    <skos:definition xml:lang="en">Where possible, public administrations should seek to streamline and simplify their
      administrative processes by improving them or eliminating any that does not provide public value. Administrative
      simplification can help businesses and citizens to reduce the administrative burden of complying with EU
      legislation or national obligations. Likewise, public administrations should introduce European public services
      supported by electronic means, including their interactions with other public administrations, citizens and
      businesses. Digitisation of public services should take place in accordance with the following concepts: (1).
      digital-by-default, whenever appropriate, so that there is at least one digital channel available for accessing
      and using a given European public service; (2). igital-first, which means that priority is given to using public
      services via digital channels while applying the multi-channel delivery concept and the no-wrong-door policy, i.e.
      physical and digital channels co-exist.
    </skos:definition>
    <skos:broader rdf:resource="http://data.europa.eu/Principle"/>
    <skos:inScheme rdf:resource="http://data.europa.eu/eif/"/>
    <adms:identifier>13</adms:identifier>
  </skos:Concept>

  <skos:Concept rdf:about="http://data.europa.eu/UP11">
    <skos:prefLabel xml:lang="en">Underlying Principle 11: preservation of information</skos:prefLabel>
    <skos:altLabel xml:lang="en">UP11</skos:altLabel>
    <skos:definition xml:lang="en">Legislation requires that decisions and data are stored and can be accessed for a
      specified time. This means that records18 and information in electronic form held by public administrations for
      the purpose of documenting procedures and decisions must be preserved and be converted, where necessary, to new
      media when old media become obsolete. The goal is to ensure that records and other forms of information keep their
      legibility, reliability and integrity and can be accessed as long as needed subject to security and privacy
      provisions. o guarantee the long-term preservation of electronic records and other kinds of information, formats
      should be chosen to ensure long-term accessibility, including preservation of associated electronic signatures or
      seals. In this regard, the use of qualified preservation services, in line with Regulation (EU) 910/2014, can
      ensure the long-term preservation of information. For information sources owned and managed by national
      administrations, preservation is a purely national matter. For information that is not strictly national,
      preservation becomes a European issue. In that case, an appropriate ‘preservation policy’ should be applied by the
      Member States concerned, to cope with any difficulties arising if the relevant information is used under different
      jurisdictions.
    </skos:definition>
    <skos:broader rdf:resource="http://data.europa.eu/Principle"/>
    <skos:inScheme rdf:resource="http://data.europa.eu/eif/"/>
    <adms:identifier>14</adms:identifier>
  </skos:Concept>

  <skos:Concept rdf:about="http://data.europa.eu/UP12">
    <skos:prefLabel xml:lang="en">Underlying Principle 12: assessment of effectiveness and efficiency</skos:prefLabel>
    <skos:altLabel xml:lang="en">UP12</skos:altLabel>
    <skos:definition xml:lang="en">There are many ways to take stock of the value of interoperable European public
      services, including considerations such as return on investment, total cost of ownership, level of flexibility and
      adaptability, reduced administrative burden, efficiency, reduced risk, transparency, simplification, improved
      working methods, and level of user satisfaction. Various technological solutions should be evaluated when striving
      to ensure the effectiveness and efficiency of a European public service.
    </skos:definition>
    <skos:broader rdf:resource="http://data.europa.eu/Principle"/>
    <skos:inScheme rdf:resource="http://data.europa.eu/eif/"/>
    <adms:identifier>15</adms:identifier>
  </skos:Concept>

  <skos:Concept rdf:about="http://data.europa.eu/IL1">
    <skos:prefLabel xml:lang="en">Interoperability Layer 1: Interoperability governance</skos:prefLabel>
    <skos:altLabel xml:lang="en">IL1</skos:altLabel>
    <skos:definition xml:lang="en">Interoperability governance refers to decisions on interoperability frameworks,
      institutional arrangements, organisational structures, roles and responsibilities, policies, agreements and other
      aspects of ensuring and monitoring interoperability at national and EU levels.
    </skos:definition>
    <skos:broader rdf:resource="http://data.europa.eu/Layer"/>
    <skos:inScheme rdf:resource="http://data.europa.eu/eif/"/>
    <adms:identifier>16</adms:identifier>
  </skos:Concept>

  <skos:Concept rdf:about="http://data.europa.eu/IL2">
    <skos:prefLabel xml:lang="en">Interoperability Layer 2: Integrated public service governance</skos:prefLabel>
    <skos:altLabel xml:lang="en">IL2</skos:altLabel>
    <skos:definition xml:lang="en">European public services should be governed to ensure: integration, seamless
      execution, reuse of services and data, and development of new services and ‘building blocks’
    </skos:definition>
    <skos:broader rdf:resource="http://data.europa.eu/Layer"/>
    <skos:inScheme rdf:resource="http://data.europa.eu/eif/"/>
    <adms:identifier>17</adms:identifier>
  </skos:Concept>

  <skos:Concept rdf:about="http://data.europa.eu/IL3">
    <skos:prefLabel xml:lang="en">Interoperability Layer 3: Legal interoperability</skos:prefLabel>
    <skos:altLabel xml:lang="en">IL3</skos:altLabel>
    <skos:definition xml:lang="en">Legal interoperability is about ensuring that organisations operating under different
      legal frameworks, policies and strategies are able to work together.
    </skos:definition>
    <skos:broader rdf:resource="http://data.europa.eu/Layer"/>
    <skos:inScheme rdf:resource="http://data.europa.eu/eif/"/>
    <adms:identifier>18</adms:identifier>
  </skos:Concept>

  <skos:Concept rdf:about="http://data.europa.eu/IL4">
    <skos:prefLabel xml:lang="en">Interoperability Layer 4: Organisational interoperability</skos:prefLabel>
    <skos:altLabel xml:lang="en">IL4</skos:altLabel>
    <skos:definition xml:lang="en">This refers to the way in which public administrations align their business
      processes, responsibilities and expectations to achieve commonly agreed and mutually beneficial goals.
    </skos:definition>
    <skos:broader rdf:resource="http://data.europa.eu/Layer"/>
    <skos:inScheme rdf:resource="http://data.europa.eu/eif/"/>
    <adms:identifier>19</adms:identifier>
  </skos:Concept>

  <skos:Concept rdf:about="http://data.europa.eu/IL5">
    <skos:prefLabel xml:lang="en">Interoperability Layer 5: Semantic interoperability</skos:prefLabel>
    <skos:altLabel xml:lang="en">IL5</skos:altLabel>
    <skos:definition xml:lang="en">Semantic interoperability ensures that the precise format and meaning of exchanged
      data and information is preserved and understood throughout exchanges between parties, in other words ‘what is
      sent is what is understood.
    </skos:definition>
    <skos:broader rdf:resource="http://data.europa.eu/Layer"/>
    <skos:inScheme rdf:resource="http://data.europa.eu/eif/"/>
    <adms:identifier>20</adms:identifier>
  </skos:Concept>

  <skos:Concept rdf:about="http://data.europa.eu/IL6">
    <skos:prefLabel xml:lang="en">Interoperability Layer 6: Technical interoperability</skos:prefLabel>
    <skos:altLabel xml:lang="en">IL6</skos:altLabel>
    <skos:definition xml:lang="en">This covers the applications and infrastructures linking systems and services.
      Aspects of technical interoperability include interface specifications, interconnection services, data integration
      services, data presentation and exchange, and secure communication protocols.
    </skos:definition>
    <skos:broader rdf:resource="http://data.europa.eu/Layer"/>
    <skos:inScheme rdf:resource="http://data.europa.eu/eif/"/>
    <adms:identifier>21</adms:identifier>
  </skos:Concept>

  <skos:Concept rdf:about="http://data.europa.eu/BC1">
    <skos:prefLabel xml:lang="en">Basic Component 1: Coordination function</skos:prefLabel>
    <skos:altLabel xml:lang="en">BC1</skos:altLabel>
    <skos:definition xml:lang="en">The coordination function ensures that needs are identified and appropriate services
      are invoked and orchestrated to provide a European public service.
    </skos:definition>
    <skos:broader rdf:resource="http://data.europa.eu/Model"/>
    <skos:inScheme rdf:resource="http://data.europa.eu/eif/"/>
    <adms:identifier>22</adms:identifier>
  </skos:Concept>

  <skos:Concept rdf:about="http://data.europa.eu/BC2">
    <skos:prefLabel xml:lang="en">Basic Component 2: Internal information sources and services</skos:prefLabel>
    <skos:altLabel xml:lang="en">BC2</skos:altLabel>
    <skos:definition xml:lang="en">Information sources (base registries, open data portals, and other authoritative
      sources of information) and services available not only inside the administrative system but also in the external
      environment can be used to create integrated public services as building blocks. Building blocks (information
      sources and services) should make their data or functionality accessible using service-oriented approaches.
    </skos:definition>
    <skos:broader rdf:resource="http://data.europa.eu/Model"/>
    <skos:inScheme rdf:resource="http://data.europa.eu/eif/"/>
    <adms:identifier>23</adms:identifier>
  </skos:Concept>

  <skos:Concept rdf:about="http://data.europa.eu/BC3">
    <skos:prefLabel xml:lang="en">Basic Component 3: Base registries</skos:prefLabel>
    <skos:altLabel xml:lang="en">BC3</skos:altLabel>
    <skos:definition xml:lang="en">Base registries are the cornerstone of European public service delivery. A base
      registry is a trusted and authoritative source of information which can and should be digitally reused by others,
      where one organisation is responsible and accountable for the collection, use, updating and preservation of
      information.
    </skos:definition>
    <skos:broader rdf:resource="http://data.europa.eu/Model"/>
    <skos:inScheme rdf:resource="http://data.europa.eu/eif/"/>
    <adms:identifier>24</adms:identifier>
  </skos:Concept>

  <skos:Concept rdf:about="http://data.europa.eu/BC4">
    <skos:prefLabel xml:lang="en">Basic Component 4: Open data</skos:prefLabel>
    <skos:altLabel xml:lang="en">BC4</skos:altLabel>
    <skos:definition xml:lang="en">The Directive on the reuse of public sector information provides a common legal
      framework for reuse of public sector data. The focus is on releasing machine-readable data for use by others to
      stimulate transparency, fair competition, innovation and a data-driven economy. To ensure a level playing field,
      the opening and reuse of data must be non-discriminatory, meaning that data must be interoperable so that can be
      found, discovered and processed.
    </skos:definition>
    <skos:broader rdf:resource="http://data.europa.eu/Model"/>
    <skos:inScheme rdf:resource="http://data.europa.eu/eif/"/>
    <adms:identifier>25</adms:identifier>
  </skos:Concept>

  <skos:Concept rdf:about="http://data.europa.eu/BC5">
    <skos:prefLabel xml:lang="en">Basic Component 5: Catalogues</skos:prefLabel>
    <skos:altLabel xml:lang="en">BC5</skos:altLabel>
    <skos:definition xml:lang="en">Catalogues help others to find reusable resources (e.g. services, data, software,
      data models). Various types of catalogue exist, e.g. directories of services, libraries of software components,
      open data portals, registries of base registries, metadata catalogues, catalogues of standards, specifications and
      guidelines. Commonly agreed descriptions of the services, data, registries and interoperable solutions published
      in catalogues are needed to enable interoperability between catalogues.
    </skos:definition>
    <skos:broader rdf:resource="http://data.europa.eu/Model"/>
    <skos:inScheme rdf:resource="http://data.europa.eu/eif/"/>
    <adms:identifier>26</adms:identifier>
  </skos:Concept>

  <skos:Concept rdf:about="http://data.europa.eu/BC6">
    <skos:prefLabel xml:lang="en">Basic Component 6: External information sources and services</skos:prefLabel>
    <skos:altLabel xml:lang="en">BC6</skos:altLabel>
    <skos:definition xml:lang="en">Public administrations need to exploit services delivered outside their
      organisational boundaries by third parties, such as payment services provided by financial institutions or
      connectivity services provided by telecommunications providers. They need also to exploit external information
      sources such as open data and data from international organisations, chambers of commerce, etc. Moreover, useful
      data can be collected through the Internet of Things (e.g. sensors) and social web applications.
    </skos:definition>
    <skos:broader rdf:resource="http://data.europa.eu/Model"/>
    <skos:inScheme rdf:resource="http://data.europa.eu/eif/"/>
    <adms:identifier>27</adms:identifier>
  </skos:Concept>

  <skos:Concept rdf:about="http://data.europa.eu/BC7">
    <skos:prefLabel xml:lang="en">Basic Component 7: Security and privacy</skos:prefLabel>
    <skos:altLabel xml:lang="en">BC7</skos:altLabel>
    <skos:definition xml:lang="en">Security and privacy are primary concerns in the provision of public services.
    </skos:definition>
    <skos:broader rdf:resource="http://data.europa.eu/Model"/>
    <skos:inScheme rdf:resource="http://data.europa.eu/eif/"/>
    <adms:identifier>28</adms:identifier>
  </skos:Concept>

  <skos:Concept rdf:about="http://data.europa.eu/Rec1">
    <skos:prefLabel xml:lang="en">Recommendation 1</skos:prefLabel>
    <skos:altLabel xml:lang="en">Rec1</skos:altLabel>
    <skos:definition xml:lang="en">Ensure that national interoperability frameworks and interoperability strategies are
      aligned with the EIF and, if needed, tailor and extend them to address the national context and needs.
    </skos:definition>
    <skos:broader rdf:resource="http://data.europa.eu/Recommendation"/>
    <skos:related rdf:resource="http://data.europa.eu/UP1"/>
    <skos:inScheme rdf:resource="http://data.europa.eu/eif/"/>
    <adms:identifier>29</adms:identifier>
  </skos:Concept>

  <skos:Concept rdf:about="http://data.europa.eu/Rec2">
    <skos:prefLabel xml:lang="en">Recommendation 2</skos:prefLabel>
    <skos:altLabel xml:lang="en">Rec2</skos:altLabel>
    <skos:definition xml:lang="en">Publish the data you own as open data unless certain restrictions apply.
    </skos:definition>
    <skos:broader rdf:resource="http://data.europa.eu/Recommendation"/>
    <skos:related rdf:resource="http://data.europa.eu/UP2"/>
    <skos:inScheme rdf:resource="http://data.europa.eu/eif/"/>
    <adms:identifier>30</adms:identifier>
  </skos:Concept>

  <skos:Concept rdf:about="http://data.europa.eu/Rec3">
    <skos:prefLabel xml:lang="en">Recommendation 3</skos:prefLabel>
    <skos:altLabel xml:lang="en">Rec3</skos:altLabel>
    <skos:definition xml:lang="en">Ensure a level playing field for open source software and demonstrate active and fair
      consideration of using open source software, taking into account the total cost of ownership of the solution.
    </skos:definition>
    <skos:broader rdf:resource="http://data.europa.eu/Recommendation"/>
    <skos:related rdf:resource="http://data.europa.eu/UP2"/>
    <skos:inScheme rdf:resource="http://data.europa.eu/eif/"/>
    <adms:identifier>31</adms:identifier>
  </skos:Concept>

  <skos:Concept rdf:about="http://data.europa.eu/Rec4">
    <skos:prefLabel xml:lang="en">Recommendation 4</skos:prefLabel>
    <skos:altLabel xml:lang="en">Rec4</skos:altLabel>
    <skos:definition xml:lang="en">Give preference to open specifications, taking due account of the coverage of
      functional needs, maturity and market support and innovation.
    </skos:definition>
    <skos:broader rdf:resource="http://data.europa.eu/Recommendation"/>
    <skos:related rdf:resource="http://data.europa.eu/UP2"/>
    <skos:inScheme rdf:resource="http://data.europa.eu/eif/"/>
    <adms:identifier>32</adms:identifier>
  </skos:Concept>

  <skos:Concept rdf:about="http://data.europa.eu/Rec5">
    <skos:prefLabel xml:lang="en">Recommendation 5</skos:prefLabel>
    <skos:altLabel xml:lang="en">Rec5</skos:altLabel>
    <skos:definition xml:lang="en">Ensure internal visibility and provide external interfaces for European public
      services.
    </skos:definition>
    <skos:broader rdf:resource="http://data.europa.eu/Recommendation"/>
    <skos:related rdf:resource="http://data.europa.eu/UP3"/>
    <skos:inScheme rdf:resource="http://data.europa.eu/eif/"/>
    <adms:identifier>33</adms:identifier>
  </skos:Concept>

  <skos:Concept rdf:about="http://data.europa.eu/Rec6">
    <skos:prefLabel xml:lang="en">Recommendation 6</skos:prefLabel>
    <skos:altLabel xml:lang="en">Rec6</skos:altLabel>
    <skos:definition xml:lang="en">Reuse and share solutions, and cooperate in the development of joint solutions when
      implementing European public services.
    </skos:definition>
    <skos:broader rdf:resource="http://data.europa.eu/Recommendation"/>
    <skos:related rdf:resource="http://data.europa.eu/UP4"/>
    <skos:inScheme rdf:resource="http://data.europa.eu/eif/"/>
    <adms:identifier>34</adms:identifier>
  </skos:Concept>

  <skos:Concept rdf:about="http://data.europa.eu/Rec7">
    <skos:prefLabel xml:lang="en">Recommendation 7</skos:prefLabel>
    <skos:altLabel xml:lang="en">Rec7</skos:altLabel>
    <skos:definition xml:lang="en">Reuse and share information and data when implementing European public services,
      unless certain privacy or confidentiality restrictions apply.
    </skos:definition>
    <skos:broader rdf:resource="http://data.europa.eu/Recommendation"/>
    <skos:related rdf:resource="http://data.europa.eu/UP4"/>
    <skos:inScheme rdf:resource="http://data.europa.eu/eif/"/>
    <adms:identifier>35</adms:identifier>
  </skos:Concept>

  <skos:Concept rdf:about="http://data.europa.eu/Rec8">
    <skos:prefLabel xml:lang="en">Recommendation 8</skos:prefLabel>
    <skos:altLabel xml:lang="en">Rec8</skos:altLabel>
    <skos:definition xml:lang="en">Do not impose any technological solutions on citizens, businesses and other
      administrations that are technology-specific or disproportionate to their real needs..
    </skos:definition>
    <skos:broader rdf:resource="http://data.europa.eu/Recommendation"/>
    <skos:related rdf:resource="http://data.europa.eu/UP5"/>
    <skos:inScheme rdf:resource="http://data.europa.eu/eif/"/>
    <adms:identifier>36</adms:identifier>
  </skos:Concept>

  <skos:Concept rdf:about="http://data.europa.eu/Rec9">
    <skos:prefLabel xml:lang="en">Recommendation 9</skos:prefLabel>
    <skos:altLabel xml:lang="en">Rec9</skos:altLabel>
    <skos:definition xml:lang="en">Ensure data portability, namely that data is easily transferable between systems and
      applications supporting the implementation and evolution of European public services without unjustified
      restrictions, if legally possible.
    </skos:definition>
    <skos:broader rdf:resource="http://data.europa.eu/Recommendation"/>
    <skos:related rdf:resource="http://data.europa.eu/UP5"/>
    <skos:inScheme rdf:resource="http://data.europa.eu/eif/"/>
    <adms:identifier>37</adms:identifier>
  </skos:Concept>

  <skos:Concept rdf:about="http://data.europa.eu/Rec10">
    <skos:prefLabel xml:lang="en">Recommendation 10</skos:prefLabel>
    <skos:altLabel xml:lang="en">Rec10</skos:altLabel>
    <skos:definition xml:lang="en">Use multiple channels to provide the European public service, to ensure that users
      can select the channel that best suits their needs.
    </skos:definition>
    <skos:broader rdf:resource="http://data.europa.eu/Recommendation"/>
    <skos:related rdf:resource="http://data.europa.eu/UP6"/>
    <skos:inScheme rdf:resource="http://data.europa.eu/eif/"/>
    <adms:identifier>38</adms:identifier>
  </skos:Concept>

  <skos:Concept rdf:about="http://data.europa.eu/Rec11">
    <skos:prefLabel xml:lang="en">Recommendation 11</skos:prefLabel>
    <skos:altLabel xml:lang="en">Rec11</skos:altLabel>
    <skos:definition xml:lang="en">Provide a single point of contact in order to hide internal administrative complexity
      and facilitate users’ access to European public services.
    </skos:definition>
    <skos:broader rdf:resource="http://data.europa.eu/Recommendation"/>
    <skos:related rdf:resource="http://data.europa.eu/UP6"/>
    <skos:inScheme rdf:resource="http://data.europa.eu/eif/"/>
    <adms:identifier>39</adms:identifier>
  </skos:Concept>

  <skos:Concept rdf:about="http://data.europa.eu/Rec12">
    <skos:prefLabel xml:lang="en">Recommendation 12</skos:prefLabel>
    <skos:altLabel xml:lang="en">Rec12</skos:altLabel>
    <skos:definition xml:lang="en">Put in place mechanisms to involve users in analysis, design, assessment and further
      development of European public services.
    </skos:definition>
    <skos:broader rdf:resource="http://data.europa.eu/Recommendation"/>
    <skos:related rdf:resource="http://data.europa.eu/UP6"/>
    <skos:inScheme rdf:resource="http://data.europa.eu/eif/"/>
    <adms:identifier>40</adms:identifier>
  </skos:Concept>

  <skos:Concept rdf:about="http://data.europa.eu/Rec13">
    <skos:prefLabel xml:lang="en">Recommendation 13</skos:prefLabel>
    <skos:altLabel xml:lang="en">Rec13</skos:altLabel>
    <skos:definition xml:lang="en">As far as possible under the legislation in force, ask users of European public
      services once-only and relevant-only information.
    </skos:definition>
    <skos:broader rdf:resource="http://data.europa.eu/Recommendation"/>
    <skos:related rdf:resource="http://data.europa.eu/UP6"/>
    <skos:inScheme rdf:resource="http://data.europa.eu/eif/"/>
    <adms:identifier>41</adms:identifier>
  </skos:Concept>

  <skos:Concept rdf:about="http://data.europa.eu/Rec14">
    <skos:prefLabel xml:lang="en">Recommendation 14</skos:prefLabel>
    <skos:altLabel xml:lang="en">Rec14</skos:altLabel>
    <skos:definition xml:lang="en">Ensure that all European public services are accessible to all citizens, including
      persons with disabilities, the elderly and other disadvantaged groups. For digital public services, public
      administrations should comply with e-accessibility specifications that are widely recognised at European or
      international level.
    </skos:definition>
    <skos:broader rdf:resource="http://data.europa.eu/Recommendation"/>
    <skos:related rdf:resource="http://data.europa.eu/UP7"/>
    <skos:inScheme rdf:resource="http://data.europa.eu/eif/"/>
    <adms:identifier>42</adms:identifier>
  </skos:Concept>

  <skos:Concept rdf:about="http://data.europa.eu/Rec15">
    <skos:prefLabel xml:lang="en">Recommendation 15</skos:prefLabel>
    <skos:altLabel xml:lang="en">Rec15</skos:altLabel>
    <skos:definition xml:lang="en">Define a common security and privacy framework and establish processes for public
      services to ensure secure and trustworthy data exchange between public administrations and in interactions with
      citizens and businesses
    </skos:definition>
    <skos:broader rdf:resource="http://data.europa.eu/Recommendation"/>
    <skos:related rdf:resource="http://data.europa.eu/UP8"/>
    <skos:inScheme rdf:resource="http://data.europa.eu/eif/"/>
    <adms:identifier>43</adms:identifier>
  </skos:Concept>

  <skos:Concept rdf:about="http://data.europa.eu/Rec16">
    <skos:prefLabel xml:lang="en">Recommendation 16</skos:prefLabel>
    <skos:altLabel xml:lang="en">Rec16</skos:altLabel>
    <skos:definition xml:lang="en">Use information systems and technical architectures that cater for multilingualism
      when establishing a European public service. Decide on the level of multilingualism support based on the needs of
      the expected users.
    </skos:definition>
    <skos:broader rdf:resource="http://data.europa.eu/Recommendation"/>
    <skos:related rdf:resource="http://data.europa.eu/UP9"/>
    <skos:inScheme rdf:resource="http://data.europa.eu/eif/"/>
    <adms:identifier>44</adms:identifier>
  </skos:Concept>

  <skos:Concept rdf:about="http://data.europa.eu/Rec17">
    <skos:prefLabel xml:lang="en">Recommendation 17</skos:prefLabel>
    <skos:altLabel xml:lang="en">Rec17</skos:altLabel>
    <skos:definition xml:lang="en">Simplify processes and use digital channels whenever appropriate for the delivery of
      European public services, to respond promptly and with high quality to users’ requests and reduce the
      administrative burden on public administrations, businesses and citizens.
    </skos:definition>
    <skos:broader rdf:resource="http://data.europa.eu/Recommendation"/>
    <skos:related rdf:resource="http://data.europa.eu/UP10"/>
    <skos:inScheme rdf:resource="http://data.europa.eu/eif/"/>
    <adms:identifier>45</adms:identifier>
  </skos:Concept>

  <skos:Concept rdf:about="http://data.europa.eu/Rec18">
    <skos:prefLabel xml:lang="en">Recommendation 18</skos:prefLabel>
    <skos:altLabel xml:lang="en">Rec18</skos:altLabel>
    <skos:definition xml:lang="en">Formulate a long-term preservation policy for information related to European public
      services and especially for information that is exchanged across borders.
    </skos:definition>
    <skos:broader rdf:resource="http://data.europa.eu/Recommendation"/>
    <skos:related rdf:resource="http://data.europa.eu/UP11"/>
    <skos:inScheme rdf:resource="http://data.europa.eu/eif/"/>
    <adms:identifier>46</adms:identifier>
  </skos:Concept>

  <skos:Concept rdf:about="http://data.europa.eu/Rec19">
    <skos:prefLabel xml:lang="en">Recommendation 19</skos:prefLabel>
    <skos:altLabel xml:lang="en">Rec19</skos:altLabel>
    <skos:definition xml:lang="en">Evaluate the effectiveness and efficiency of different interoperability solutions and
      technological options considering user needs, proportionality and balance between costs and benefits.
    </skos:definition>
    <skos:broader rdf:resource="http://data.europa.eu/Recommendation"/>
    <skos:related rdf:resource="http://data.europa.eu/UP12"/>
    <skos:inScheme rdf:resource="http://data.europa.eu/eif/"/>
    <adms:identifier>47</adms:identifier>
  </skos:Concept>

  <skos:Concept rdf:about="http://data.europa.eu/Rec20">
    <skos:prefLabel xml:lang="en">Recommendation 20</skos:prefLabel>
    <skos:altLabel xml:lang="en">Rec20</skos:altLabel>
    <skos:definition xml:lang="en">Ensure holistic governance of interoperability activities across administrative
      levels and sectors.
    </skos:definition>
    <skos:broader rdf:resource="http://data.europa.eu/Recommendation"/>
    <skos:related rdf:resource="http://data.europa.eu/IL1"/>
    <skos:inScheme rdf:resource="http://data.europa.eu/eif/"/>
    <adms:identifier>48</adms:identifier>
  </skos:Concept>

  <skos:Concept rdf:about="http://data.europa.eu/Rec21">
    <skos:prefLabel xml:lang="en">Recommendation 21</skos:prefLabel>
    <skos:altLabel xml:lang="en">Rec21</skos:altLabel>
    <skos:definition xml:lang="en">Put in place processes to select relevant standards and specifications, evaluate
      them, monitor their implementation, check compliance and test their interoperability.
    </skos:definition>
    <skos:broader rdf:resource="http://data.europa.eu/Recommendation"/>
    <skos:related rdf:resource="http://data.europa.eu/IL1"/>
    <skos:inScheme rdf:resource="http://data.europa.eu/eif/"/>
    <adms:identifier>49</adms:identifier>
  </skos:Concept>

  <skos:Concept rdf:about="http://data.europa.eu/Rec22">
    <skos:prefLabel xml:lang="en">Recommendation 22</skos:prefLabel>
    <skos:altLabel xml:lang="en">Rec22</skos:altLabel>
    <skos:definition xml:lang="en">Use a structured, transparent, objective and common approach to assessing and
      selecting standards and specifications. Take into account relevant EU recommendations and seek to make the
      approach consistent across borders.
    </skos:definition>
    <skos:broader rdf:resource="http://data.europa.eu/Recommendation"/>
    <skos:related rdf:resource="http://data.europa.eu/IL1"/>
    <skos:inScheme rdf:resource="http://data.europa.eu/eif/"/>
    <adms:identifier>50</adms:identifier>
  </skos:Concept>

  <skos:Concept rdf:about="http://data.europa.eu/Rec23">
    <skos:prefLabel xml:lang="en">Recommendation 23</skos:prefLabel>
    <skos:altLabel xml:lang="en">Rec23</skos:altLabel>
    <skos:definition xml:lang="en">Consult relevant catalogues of standards, specifications and guidelines at national
      and EU level, in accordance with your NIF and relevant DIFs, when procuring and developing ICT solutions.
    </skos:definition>
    <skos:broader rdf:resource="http://data.europa.eu/Recommendation"/>
    <skos:related rdf:resource="http://data.europa.eu/IL1"/>
    <skos:inScheme rdf:resource="http://data.europa.eu/eif/"/>
    <adms:identifier>51</adms:identifier>
  </skos:Concept>

  <skos:Concept rdf:about="http://data.europa.eu/Rec24">
    <skos:prefLabel xml:lang="en">Recommendation 24</skos:prefLabel>
    <skos:altLabel xml:lang="en">Rec24</skos:altLabel>
    <skos:definition xml:lang="en">Actively participate in standardisation work relevant to your needs to ensure your
      requirements are met.
    </skos:definition>
    <skos:broader rdf:resource="http://data.europa.eu/Recommendation"/>
    <skos:related rdf:resource="http://data.europa.eu/IL1"/>
    <skos:inScheme rdf:resource="http://data.europa.eu/eif/"/>
    <adms:identifier>52</adms:identifier>
  </skos:Concept>

  <skos:Concept rdf:about="http://data.europa.eu/Rec25">
    <skos:prefLabel xml:lang="en">Recommendation 25</skos:prefLabel>
    <skos:altLabel xml:lang="en">Rec25</skos:altLabel>
    <skos:definition xml:lang="en">Ensure interoperability and coordination over time when operating and delivering
      integrated public services by putting in place the necessary governance structure.
    </skos:definition>
    <skos:broader rdf:resource="http://data.europa.eu/Recommendation"/>
    <skos:related rdf:resource="http://data.europa.eu/IL2"/>
    <skos:inScheme rdf:resource="http://data.europa.eu/eif/"/>
    <adms:identifier>53</adms:identifier>
  </skos:Concept>

  <skos:Concept rdf:about="http://data.europa.eu/Rec26">
    <skos:prefLabel xml:lang="en">Recommendation 26</skos:prefLabel>
    <skos:altLabel xml:lang="en">Rec26</skos:altLabel>
    <skos:definition xml:lang="en">Establish interoperability agreements in all layers, complemented by operational
      agreements and change management procedures.
    </skos:definition>
    <skos:broader rdf:resource="http://data.europa.eu/Recommendation"/>
    <skos:related rdf:resource="http://data.europa.eu/IL2"/>
    <skos:inScheme rdf:resource="http://data.europa.eu/eif/"/>
    <adms:identifier>54</adms:identifier>
  </skos:Concept>

  <skos:Concept rdf:about="http://data.europa.eu/Rec27">
    <skos:prefLabel xml:lang="en">Recommendation 27</skos:prefLabel>
    <skos:altLabel xml:lang="en">Rec27</skos:altLabel>
    <skos:definition xml:lang="en">Ensure that legislation is screened by means of ‘interoperability checks’, to
      identify any barriers to interoperability. When drafting legislation to establish a European public service, seek
      to make it consistent with relevant legislation, perform a ‘digital check’ and consider data protection
      requirementss.
    </skos:definition>
    <skos:broader rdf:resource="http://data.europa.eu/Recommendation"/>
    <skos:related rdf:resource="http://data.europa.eu/IL3"/>
    <skos:inScheme rdf:resource="http://data.europa.eu/eif/"/>
    <adms:identifier>55</adms:identifier>
  </skos:Concept>

  <skos:Concept rdf:about="http://data.europa.eu/Rec28">
    <skos:prefLabel xml:lang="en">Recommendation 28</skos:prefLabel>
    <skos:altLabel xml:lang="en">Rec28</skos:altLabel>
    <skos:definition xml:lang="en">Document your business processes using commonly accepted modelling techniques and
      agree on how these processes should be aligned to deliver a European public service.
    </skos:definition>
    <skos:broader rdf:resource="http://data.europa.eu/Recommendation"/>
    <skos:related rdf:resource="http://data.europa.eu/IL4"/>
    <skos:inScheme rdf:resource="http://data.europa.eu/eif/"/>
    <adms:identifier>56</adms:identifier>
  </skos:Concept>

  <skos:Concept rdf:about="http://data.europa.eu/Rec29">
    <skos:prefLabel xml:lang="en">Recommendation 29</skos:prefLabel>
    <skos:altLabel xml:lang="en">Rec29</skos:altLabel>
    <skos:definition xml:lang="en">Clarify and formalise your organisational relationships for establishing and
      operating European public services.
    </skos:definition>
    <skos:broader rdf:resource="http://data.europa.eu/Recommendation"/>
    <skos:related rdf:resource="http://data.europa.eu/IL4"/>
    <skos:inScheme rdf:resource="http://data.europa.eu/eif/"/>
    <adms:identifier>57</adms:identifier>
  </skos:Concept>

  <skos:Concept rdf:about="http://data.europa.eu/Rec30">
    <skos:prefLabel xml:lang="en">Recommendation 30</skos:prefLabel>
    <skos:altLabel xml:lang="en">Rec30</skos:altLabel>
    <skos:definition xml:lang="en">Perceive data and information as a public asset that should be appropriately
      generated, collected, managed, shared, protected and preserved.
    </skos:definition>
    <skos:broader rdf:resource="http://data.europa.eu/Recommendation"/>
    <skos:related rdf:resource="http://data.europa.eu/IL5"/>
    <skos:inScheme rdf:resource="http://data.europa.eu/eif/"/>
    <adms:identifier>58</adms:identifier>
  </skos:Concept>

  <skos:Concept rdf:about="http://data.europa.eu/Rec31">
    <skos:prefLabel xml:lang="en">Recommendation 31</skos:prefLabel>
    <skos:altLabel xml:lang="en">Rec31</skos:altLabel>
    <skos:definition xml:lang="en">Put in place an information management strategy at the highest possible level to
      avoid fragmentation and duplication. Management of metadata, master data and reference data should be prioritised.
    </skos:definition>
    <skos:broader rdf:resource="http://data.europa.eu/Recommendation"/>
    <skos:related rdf:resource="http://data.europa.eu/IL5"/>
    <skos:inScheme rdf:resource="http://data.europa.eu/eif/"/>
    <adms:identifier>59</adms:identifier>
  </skos:Concept>

  <skos:Concept rdf:about="http://data.europa.eu/Rec32">
    <skos:prefLabel xml:lang="en">Recommendation 32</skos:prefLabel>
    <skos:altLabel xml:lang="en">Rec32</skos:altLabel>
    <skos:definition xml:lang="en">Support the establishment of sector-specific and cross-sectoral communities that aim
      to create open information specifications and encourage relevant communities to share their results on national
      and European platforms.
    </skos:definition>
    <skos:broader rdf:resource="http://data.europa.eu/Recommendation"/>
    <skos:related rdf:resource="http://data.europa.eu/IL5"/>
    <skos:inScheme rdf:resource="http://data.europa.eu/eif/"/>
    <adms:identifier>60</adms:identifier>
  </skos:Concept>

  <skos:Concept rdf:about="http://data.europa.eu/Rec33">
    <skos:prefLabel xml:lang="en">Recommendation 33</skos:prefLabel>
    <skos:altLabel xml:lang="en">Rec33</skos:altLabel>
    <skos:definition xml:lang="en">Use open specifications, where available, to ensure technical interoperability when
      establishing European public services.
    </skos:definition>
    <skos:broader rdf:resource="http://data.europa.eu/Recommendation"/>
    <skos:related rdf:resource="http://data.europa.eu/IL6"/>
    <skos:inScheme rdf:resource="http://data.europa.eu/eif/"/>
    <adms:identifier>61</adms:identifier>
  </skos:Concept>

  <skos:Concept rdf:about="http://data.europa.eu/Rec34">
    <skos:prefLabel xml:lang="en">Recommendation 34</skos:prefLabel>
    <skos:altLabel xml:lang="en">Rec34</skos:altLabel>
    <skos:definition xml:lang="en">Use the conceptual model for European public services to design new services or
      reengineer existing ones and reuse, whenever possible, existing service and data components.
    </skos:definition>
    <skos:broader rdf:resource="http://data.europa.eu/Recommendation"/>
    <skos:related rdf:resource="http://data.europa.eu/Model"/>
    <skos:inScheme rdf:resource="http://data.europa.eu/eif/"/>
    <adms:identifier>62</adms:identifier>
  </skos:Concept>

  <skos:Concept rdf:about="http://data.europa.eu/Rec35">
    <skos:prefLabel xml:lang="en">Recommendation 35</skos:prefLabel>
    <skos:altLabel xml:lang="en">Rec35</skos:altLabel>
    <skos:definition xml:lang="en">Decide on a common scheme for interconnecting loosely coupled service components and
      put in place and maintain the necessary infrastructure for establishing and maintaining European public services.
    </skos:definition>
    <skos:broader rdf:resource="http://data.europa.eu/Recommendation"/>
    <skos:related rdf:resource="http://data.europa.eu/Model"/>
    <skos:inScheme rdf:resource="http://data.europa.eu/eif/"/>
    <adms:identifier>63</adms:identifier>
  </skos:Concept>

  <skos:Concept rdf:about="http://data.europa.eu/Rec36">
    <skos:prefLabel xml:lang="en">Recommendation 36</skos:prefLabel>
    <skos:altLabel xml:lang="en">Rec36</skos:altLabel>
    <skos:definition xml:lang="en">Develop a shared infrastructure of reusable services and information sources that can
      be used by all public administrations.
    </skos:definition>
    <skos:broader rdf:resource="http://data.europa.eu/Recommendation"/>
    <skos:related rdf:resource="http://data.europa.eu/BC2"/>
    <skos:inScheme rdf:resource="http://data.europa.eu/eif/"/>
    <adms:identifier>64</adms:identifier>
  </skos:Concept>

  <skos:Concept rdf:about="http://data.europa.eu/Rec37">
    <skos:prefLabel xml:lang="en">Recommendation 37</skos:prefLabel>
    <skos:altLabel xml:lang="en">Rec37</skos:altLabel>
    <skos:definition xml:lang="en">Make authoritative sources of information available to others while implementing
      access and control mechanisms to ensure security and privacy in accordance with the relevant legislation.
    </skos:definition>
    <skos:broader rdf:resource="http://data.europa.eu/Recommendation"/>
    <skos:related rdf:resource="http://data.europa.eu/BC3"/>
    <skos:inScheme rdf:resource="http://data.europa.eu/eif/"/>
    <adms:identifier>65</adms:identifier>
  </skos:Concept>

  <skos:Concept rdf:about="http://data.europa.eu/Rec38">
    <skos:prefLabel xml:lang="en">Recommendation 38</skos:prefLabel>
    <skos:altLabel xml:lang="en">Rec38</skos:altLabel>
    <skos:definition xml:lang="en">Develop interfaces with base registries and authoritative sources of information,
      publish the semantic and technical means and documentation needed for others to connect and reuse available
      information.
    </skos:definition>
    <skos:broader rdf:resource="http://data.europa.eu/Recommendation"/>
    <skos:related rdf:resource="http://data.europa.eu/BC3"/>
    <skos:inScheme rdf:resource="http://data.europa.eu/eif/"/>
    <adms:identifier>66</adms:identifier>
  </skos:Concept>

  <skos:Concept rdf:about="http://data.europa.eu/Rec39">
    <skos:prefLabel xml:lang="en">Recommendation 39</skos:prefLabel>
    <skos:altLabel xml:lang="en">Rec39</skos:altLabel>
    <skos:definition xml:lang="en">Match each base registry with appropriate metadata including the description of its
      content, service assurance and responsibilities, the type of master data it keeps, conditions of access and the
      relevant licences, terminology, a glossary, and information about any master data it uses from other base
      registries.
    </skos:definition>
    <skos:broader rdf:resource="http://data.europa.eu/Recommendation"/>
    <skos:related rdf:resource="http://data.europa.eu/BC3"/>
    <skos:inScheme rdf:resource="http://data.europa.eu/eif/"/>
    <adms:identifier>67</adms:identifier>
  </skos:Concept>

  <skos:Concept rdf:about="http://data.europa.eu/Rec40">
    <skos:prefLabel xml:lang="en">Recommendation 40</skos:prefLabel>
    <skos:altLabel xml:lang="en">Rec40</skos:altLabel>
    <skos:definition xml:lang="en">Create and follow data quality assurance plans for base registries and related master
      data.
    </skos:definition>
    <skos:broader rdf:resource="http://data.europa.eu/Recommendation"/>
    <skos:related rdf:resource="http://data.europa.eu/BC3"/>
    <skos:inScheme rdf:resource="http://data.europa.eu/eif/"/>
    <adms:identifier>68</adms:identifier>
  </skos:Concept>

  <skos:Concept rdf:about="http://data.europa.eu/Rec41">
    <skos:prefLabel xml:lang="en">Recommendation 41</skos:prefLabel>
    <skos:altLabel xml:lang="en">Rec41</skos:altLabel>
    <skos:definition xml:lang="en">Establish procedures and processes to integrate the opening of data in your common
      business processes, working routines, and in the development of new information systems.
    </skos:definition>
    <skos:broader rdf:resource="http://data.europa.eu/Recommendation"/>
    <skos:related rdf:resource="http://data.europa.eu/BC4"/>
    <skos:inScheme rdf:resource="http://data.europa.eu/eif/"/>
    <adms:identifier>69</adms:identifier>
  </skos:Concept>

  <skos:Concept rdf:about="http://data.europa.eu/Rec42">
    <skos:prefLabel xml:lang="en">Recommendation 42</skos:prefLabel>
    <skos:altLabel xml:lang="en">Rec42</skos:altLabel>
    <skos:definition xml:lang="en">Publish open data in machine-readable, non-proprietary formats. Ensure that open data
      is accompanied by high quality, machine-readable metadata in non-proprietary formats, including a description of
      their content, the way data is collected and its level of quality and the licence terms under which it is made
      available. The use of common vocabularies for expressing metadata is recommended.
    </skos:definition>
    <skos:broader rdf:resource="http://data.europa.eu/Recommendation"/>
    <skos:related rdf:resource="http://data.europa.eu/BC4"/>
    <skos:inScheme rdf:resource="http://data.europa.eu/eif/"/>
    <adms:identifier>70</adms:identifier>
  </skos:Concept>

  <skos:Concept rdf:about="http://data.europa.eu/Rec43">
    <skos:prefLabel xml:lang="en">Recommendation 43</skos:prefLabel>
    <skos:altLabel xml:lang="en">Rec43</skos:altLabel>
    <skos:definition xml:lang="en">Communicate clearly the right to access and reuse open data. The legal regimes for
      facilitating access and reuse, such as licences, should be standardised as much as possible.
    </skos:definition>
    <skos:broader rdf:resource="http://data.europa.eu/Recommendation"/>
    <skos:related rdf:resource="http://data.europa.eu/BC4"/>
    <skos:inScheme rdf:resource="http://data.europa.eu/eif/"/>
    <adms:identifier>71</adms:identifier>
  </skos:Concept>

  <skos:Concept rdf:about="http://data.europa.eu/Rec44">
    <skos:prefLabel xml:lang="en">Recommendation 44</skos:prefLabel>
    <skos:altLabel xml:lang="en">Rec44</skos:altLabel>
    <skos:definition xml:lang="en">Put in place catalogues of public services, public data, and interoperability
      solutions and use common models for describing them.
    </skos:definition>
    <skos:broader rdf:resource="http://data.europa.eu/Recommendation"/>
    <skos:related rdf:resource="http://data.europa.eu/BC5"/>
    <skos:inScheme rdf:resource="http://data.europa.eu/eif/"/>
    <adms:identifier>72</adms:identifier>
  </skos:Concept>

  <skos:Concept rdf:about="http://data.europa.eu/Rec45">
    <skos:prefLabel xml:lang="en">Recommendation 45</skos:prefLabel>
    <skos:altLabel xml:lang="en">Rec45</skos:altLabel>
    <skos:definition xml:lang="en">Where useful and feasible to do so, use external information sources and services
      while developing European public services.
    </skos:definition>
    <skos:broader rdf:resource="http://data.europa.eu/Recommendation"/>
    <skos:related rdf:resource="http://data.europa.eu/BC6"/>
    <skos:inScheme rdf:resource="http://data.europa.eu/eif/"/>
    <adms:identifier>73</adms:identifier>
  </skos:Concept>

  <skos:Concept rdf:about="http://data.europa.eu/Rec46">
    <skos:prefLabel xml:lang="en">Recommendation 46</skos:prefLabel>
    <skos:altLabel xml:lang="en">Rec46</skos:altLabel>
    <skos:definition xml:lang="en">Consider the specific security and privacy requirements and identify measures for the
      provision of each public service according to risk management plans.
    </skos:definition>
    <skos:broader rdf:resource="http://data.europa.eu/Recommendation"/>
    <skos:related rdf:resource="http://data.europa.eu/BC7"/>
    <skos:inScheme rdf:resource="http://data.europa.eu/eif/"/>
    <adms:identifier>74</adms:identifier>
  </skos:Concept>

  <skos:Concept rdf:about="http://data.europa.eu/Rec47">
    <skos:prefLabel xml:lang="en">Recommendation 47</skos:prefLabel>
    <skos:altLabel xml:lang="en">Rec47</skos:altLabel>
    <skos:definition xml:lang="en">Use trust services according to the Regulation on eID and Trust Services as
      mechanisms that ensure secure and protected data exchange in public services.
    </skos:definition>
    <skos:broader rdf:resource="http://data.europa.eu/Recommendation"/>
    <skos:related rdf:resource="http://data.europa.eu/BC7"/>
    <skos:inScheme rdf:resource="http://data.europa.eu/eif/"/>
    <adms:identifier>75</adms:identifier>
  </skos:Concept>

  <!--
    Updates 29.06.2020.
    The base URI "http://data.europa.eu/eif" was changed to "http://data.europa.eu/eif/" (trailing slash added).

    The top concepts need to be defined and have a label. Added the 4 top concepts below but should probably move to the
    top of the list.
   -->
   <skos:Concept rdf:about="http://data.europa.eu/Principle">
     <skos:prefLabel xml:lang="en">Principle</skos:prefLabel>
     <skos:altLabel xml:lang="en">Principle</skos:altLabel>
     <skos:definition xml:lang="en"> </skos:definition>
     <skos:inScheme rdf:resource="http://data.europa.eu/eif/"/>
     <adms:identifier>0</adms:identifier>
   </skos:Concept>

   <skos:Concept rdf:about="http://data.europa.eu/Recommendation">
     <skos:prefLabel xml:lang="en">Recommendation</skos:prefLabel>
     <skos:altLabel xml:lang="en">Recommendation</skos:altLabel>
     <skos:definition xml:lang="en"> </skos:definition>
     <skos:inScheme rdf:resource="http://data.europa.eu/eif/"/>
     <adms:identifier>1</adms:identifier>
   </skos:Concept>

   <skos:Concept rdf:about="http://data.europa.eu/Layer">
     <skos:prefLabel xml:lang="en">Layer</skos:prefLabel>
     <skos:altLabel xml:lang="en">Layer</skos:altLabel>
     <skos:definition xml:lang="en"> </skos:definition>
     <skos:inScheme rdf:resource="http://data.europa.eu/eif/"/>
     <adms:identifier>2</adms:identifier>
   </skos:Concept>

   <skos:Concept rdf:about="http://data.europa.eu/Model">
     <skos:prefLabel xml:lang="en">Model</skos:prefLabel>
     <skos:altLabel xml:lang="en">Model</skos:altLabel>
     <skos:definition xml:lang="en"> </skos:definition>
     <skos:inScheme rdf:resource="http://data.europa.eu/eif/"/>
     <adms:identifier>3</adms:identifier>
   </skos:Concept>

</rdf:RDF>
